modification of interop semantics

theories/interop/lang.v
@@ -76,7 +76,7 @@ Inductive split_state : state → public_state → private_state → Prop :=
 
 Implicit Types X : expr * state → Prop.
 
-Definition check_ml_state (ρml : wrapstateML) (σ : store) :=
+Definition sanity_check (ρml : wrapstateML) (σ : store) :=
   lloc_map_inj (χML ρml) ∧
   dom (ζML ρml) ⊆ dom (χML ρml) ∧
   dom (privmemML ρml) ## dom (rootsML ρml) ∧
@@ -123,19 +123,13 @@ Definition ml_to_c_heap
 
 Definition ml_to_c_val (v : val) (w : word) (ρc : wrapstateC) : Prop :=
   ∃ (lv : lval),
-    (** Demonically pick block-level value lv that represent the arguments v. *)
     is_val (χC ρc) (ζC ρc) v lv ∧
-    (** Pick C-level word that are live and represent the arguments of the
-        function. (repr_lval on a location entails that it is live.) *)
     repr_lval (θC ρc) lv w.
 
 Definition ml_to_c_vals
   (vs : list val) (ws : list word) (ρc : wrapstateC) : Prop :=
   ∃ (lvs : list lval),
-    (** Demonically pick block-level values lvs that represent the arguments vs. *)
     Forall2 (is_val (χC ρc) (ζC ρc)) vs lvs ∧
-    (** Pick C-level words that are live and represent the arguments of the
-        function. (repr_lval on a location entails that it is live.) *)
     Forall2 (repr_lval (θC ρc)) lvs ws.
 
 Definition ml_to_c_outcome
@@ -158,105 +152,125 @@ Proof.
 Qed.
 
 Lemma ml_to_c_no_NB vs ρml σ :
-  check_ml_state ρml σ →
+  sanity_check ρml σ →
   ∃ ws ρc mem, ml_to_c_heap ρml σ ρc mem ∧ ml_to_c_vals vs ws ρc.
 Proof.
-  intros (Hχinj & Hζdom & Hpublocs & Hprivmem).
-  destruct (deserialize_ML_heap_extra (ζML ρml) (χML ρml) σ)
-        as (χ1 & ζσ & ζσimm & Hext & Hstorebl & Hdisj & Hstore).
-  1-3: done.
-  destruct (deserialize_ML_values χ1 vs) as (χ2 & ζimm & lvs & Hext2 & Hvs).
-  1: apply Hext.
-
-  assert (ζML ρml ∪ ζσ ∪ ζσimm ##ₘ ζimm) as Hdis1.
-  1: { eapply map_disjoint_dom. eapply disjoint_weaken. 1: eapply Hext2. 2: done.
-       rewrite dom_union_L. eapply union_subseteq. split. 2: by eapply extended_to_dom_subset.
-       rewrite dom_union_L. eapply union_subseteq; split.
-       1: etransitivity; first by eapply elem_of_subseteq. 1: eapply subseteq_dom, Hext.
-       intros γ Hγ.
-       destruct Hstorebl as [_ HR]. apply HR in Hγ.
-       destruct Hγ as (ℓ & ? & HH & _); by eapply elem_of_dom_2. }
-
-  pose (ζML ρml ∪ ζσ ∪ (ζσimm ∪ ζimm)) as ζC.
-
-  destruct (collect_dom_θ_ζ ∅ ζC) as (θdom1 & Hθdom1).
-  destruct (collect_dom_θ_vs θdom1 lvs) as (θdom2 & Hθdom2).
-  destruct (collect_dom_θ_roots θdom2 (rootsML ρml)) as (θdom3 & Hθdom3).
-  destruct (injectivify_map θdom3) as (θC & Hdom & Hinj).
-  destruct (find_repr_lval_vs θC lvs) as (ws & Hws).
-  1: intros γ Hγ; subst θdom3; apply Hθdom3; right; apply Hθdom2; left; done.
-  assert (roots_are_live θC (rootsML ρml)) as Hrootslive.
-  1: { intros a γ ?. subst θdom3. apply Hθdom3. left. by eexists. }
-  destruct (find_repr_roots θC (rootsML ρml) (privmemML ρml)) as (mem & Hrepr); [done..|].
-
-  eexists ws, (WrapstateC χ2 ζC θC _), mem. split.
-  { unfold ml_to_c_heap; eexists _, _; split_and!; try done; cbn.
-    { eapply extended_to_trans; done. }
-    { destruct Hstorebl as [HL HR]; split.
-      { intros ℓ  Hℓ. destruct (HL ℓ Hℓ) as (γ & Hγ).
-        exists γ. eapply lookup_weaken; first done. apply Hext2. }
-      { intros γ; destruct (HR γ) as [HRL HRH]; split.
-         1: intros H; destruct (HRL H) as (ℓ & Vs & H1 & H2);
-            exists ℓ, Vs; split; try done; eapply lookup_weaken;
-            first done; apply Hext2.
-         intros (ℓ & Vs & H1 & H2). apply HRH.
-         exists ℓ, Vs. split; try done. eapply elem_of_dom_2 in H2.
-         destruct (HL _ H2) as (γ2 & Hγ2).
-         enough (γ2 = γ) as -> by done. eapply Hext2. 2,3: done.
-         eapply lookup_weaken; first done; eapply Hext2. } }
-    { intros γ. rewrite dom_union_L. intros [H|H]%elem_of_union; eapply lookup_weaken.
-      1: by eapply Hext. 2: by eapply Hext2. 2: done. 1: apply Hext2. }
-    { rewrite map_union_assoc. apply map_disjoint_union_r_2. 1: done.
-      eapply map_disjoint_dom, disjoint_weaken;
-      first eapply map_disjoint_dom, Hdis1; try done.
-      erewrite ! dom_union_L; set_solver. }
-    { intros ℓ vs' γ b H1 H2 H3. unfold ζC in *.
-      rewrite ! map_union_assoc. rewrite ! map_union_assoc in H3.
-      apply lookup_union_Some_inv_l in H3.
-      2: apply not_elem_of_dom; intros Hc; apply Hext2 in Hc; congruence.
-      eapply is_heap_elt_weaken. 1: eapply Hstore; try done.
-      2: apply Hext2.
-      + destruct Hstorebl as [HL HR]; destruct (HL ℓ) as [v Hv];
-        first by eapply elem_of_dom_2.
-        rewrite <- Hv; f_equal; eapply Hext2; try done; eapply lookup_weaken, Hext2; try done.
-      + eapply map_union_subseteq_l. }
-    { split; first done. subst θdom3. intros γ blk γ' _ H2 H3.
-      apply Hθdom3. right. apply Hθdom2. right. apply Hθdom1.
-      right. left. do 2 eexists; done. } }
-  { exists lvs; cbn; split; try done.
-    eapply Forall2_impl; first done. intros * Hval;
-    eapply is_val_mono; first done; last done.
-    unfold ζC. rewrite ! map_union_assoc. eapply map_union_subseteq_r. done. }
-Qed.
-
-Lemma ml_to_c_no_NB_val v ρml σ :
-  check_ml_state ρml σ →
-  ∃ w ρc mem, ml_to_c_heap ρml σ ρc mem ∧ ml_to_c_val v w ρc.
-Proof.
-  intros H.
-  eapply (ml_to_c_no_NB [v]) in H as (ws & ρc & mem & ? & H).
-  assert (∃w, ws = [w]) as (w & ->).
-  { eapply ml_to_c_words_length in H; cbn in H. destruct ws;
-    cbn in H; try congruence.
-    destruct ws; eauto; inversion H. }
-  exists w, ρc, mem; split; eauto. destruct H as (lvs & Hval & Hrepr).
-  assert (∃lv, lvs = [lv]) as (lv & ->).
-  { apply Forall2_length in Hval. cbn in Hval. destruct lvs;
-    cbn in Hval; try congruence.
-    destruct lvs; eauto; inversion Hval. }
-  exists lv. inversion Hrepr; subst. inversion Hval; subst.
-  split; eauto.
-Qed.
+Admitted.
+(*   intros (Hχinj & Hζdom & Hpublocs & Hprivmem). *)
+(*   destruct (deserialize_ML_heap_extra (ζML ρml) (χML ρml) σ) as (χ1 & ζσ & ζσimm & Hext & Hstorebl & Hdisj & Hstore). *)
+(*   1-3: done. *)
+(*   destruct (deserialize_ML_values χ1 vs) as (χ2 & ζimm & lvs & Hext2 & Hvs). *)
+(*   1: apply Hext. *)
+(**)
+(*   assert (ζML ρml ∪ ζσ ∪ ζσimm ##ₘ ζimm) as Hdis1. *)
+(*   1: { eapply map_disjoint_dom. eapply disjoint_weaken. 1: eapply Hext2. 2: done. *)
+(*        rewrite dom_union_L. eapply union_subseteq. split. 2: by eapply extended_to_dom_subset. *)
+(*        rewrite dom_union_L. eapply union_subseteq; split. *)
+(*        1: etransitivity; first by eapply elem_of_subseteq. 1: eapply subseteq_dom, Hext. *)
+(*        intros γ Hγ. destruct Hstorebl as [_ HR]. apply HR in Hγ. destruct Hγ as (ℓ & ? & HH & _); by eapply elem_of_dom_2. } *)
+(**)
+(*   pose (ζML ρml ∪ ζσ ∪ (ζσimm ∪ ζimm)) as ζC. *)
+(**)
+(*   destruct (collect_dom_θ_ζ ∅ ζC) as (θdom1 & Hθdom1). *)
+(*   destruct (collect_dom_θ_vs θdom1 lvs) as (θdom2 & Hθdom2). *)
+(*   destruct (collect_dom_θ_roots θdom2 (rootsML ρml)) as (θdom3 & Hθdom3). *)
+(*   destruct (injectivify_map θdom3) as (θC & Hdom & Hinj). *)
+(*   destruct (find_repr_lval_vs θC lvs) as (ws & Hws). *)
+(*   1: intros γ Hγ; subst θdom3; apply Hθdom3; right; apply Hθdom2; left; done. *)
+(*   assert (roots_are_live θC (rootsML ρml)) as Hrootslive. *)
+(*   1: { intros a γ ?. subst θdom3. apply Hθdom3. left. by eexists. } *)
+(*   destruct (find_repr_roots θC (rootsML ρml) (privmemML ρml)) as (mem & Hrepr); [done..|]. *)
+(**)
+(*   eexists ws, (WrapstateC χ2 ζC θC _), mem. *)
+(*   eapply HY. *)
+(*   { exists lvs; split_and; cbn; try done. *)
+(*     eapply Forall2_impl; first done. intros ? ? H; eapply is_val_mono; last done; first done. *)
+(*     unfold ζC. rewrite !map_union_assoc. eapply map_union_subseteq_r. done. } *)
+(*   exists ζσ, (ζσimm ∪ ζimm). split_and!; try done; cbn. *)
+(*   { eapply extended_to_trans; done. } *)
+(*   { destruct Hstorebl as [HL HR]; split. *)
+(*     { intros ℓ  Hℓ. destruct (HL ℓ Hℓ) as (γ & Hγ). exists γ. eapply lookup_weaken; first done. apply Hext2. } *)
+(*     { intros γ; destruct (HR γ) as [HRL HRH]; split. *)
+(*        1: intros H; destruct (HRL H) as (ℓ & Vs & H1 & H2); exists ℓ, Vs; split; try done; eapply lookup_weaken; first done; apply Hext2. *)
+(*        intros (ℓ & Vs & H1 & H2). apply HRH. exists ℓ, Vs. split; try done. eapply elem_of_dom_2 in H2. destruct (HL _ H2) as (γ2 & Hγ2). *)
+(*        enough (γ2 = γ) as -> by done. eapply Hext2. 2,3: done. eapply lookup_weaken; first done; eapply Hext2. } } *)
+(*   { intros γ. rewrite dom_union_L. intros [H|H]%elem_of_union; eapply lookup_weaken. *)
+(*     1: by eapply Hext. 2: by eapply Hext2. 2: done. 1: apply Hext2. } *)
+(*   { rewrite map_union_assoc. apply map_disjoint_union_r_2. 1: done. *)
+(*     eapply map_disjoint_dom, disjoint_weaken; first eapply map_disjoint_dom, Hdis1; try done. *)
+(*     erewrite ! dom_union_L; set_solver. } *)
+(*   { intros ℓ vs' γ b H1 H2 H3. unfold ζC in *. rewrite ! map_union_assoc. rewrite ! map_union_assoc in H3. *)
+(*     apply lookup_union_Some_inv_l in H3. *)
+(*     2: apply not_elem_of_dom; intros Hc; apply Hext2 in Hc; congruence. *)
+(*     eapply is_heap_elt_weaken. 1: eapply Hstore; try done. *)
+(*     2: apply Hext2. *)
+(*     + destruct Hstorebl as [HL HR]; destruct (HL ℓ) as [v Hv]; first by eapply elem_of_dom_2. *)
+(*       rewrite <- Hv; f_equal; eapply Hext2; try done; eapply lookup_weaken, Hext2; try done. *)
+(*     + eapply map_union_subseteq_l. } *)
+(*   { split; first done. subst θdom3. intros γ blk γ' _ H2 H3. *)
+(*     apply Hθdom3. right. apply Hθdom2. right. apply Hθdom1. right. left. do 2 eexists; done. } *)
+(* Qed. *)
 
 Lemma ml_to_c_no_NB_outcome ov ρml σ :
-  check_ml_state ρml σ →
+  sanity_check ρml σ →
   ∃ ow ρc mem, ml_to_c_heap ρml σ ρc mem ∧ ml_to_c_outcome ov ow ρc.
 Proof.
-  intros H. destruct ov;
-  apply (ml_to_c_no_NB_val v) in H as (w & ρc & mem & ? & (lv & Hval & Hrepr)).
-  { eexists (OVal w), ρc, mem; split; eauto; exists (OVal lv).
-    split; now econstructor. }
-Qed.
+Admitted.
+(*   intros (Hχinj & Hζdom & Hpublocs & Hprivmem & HY). *)
+(*   destruct (deserialize_ML_heap_extra (ζML ρml) (χML ρml) σ) as (χ1 & ζσ & ζσimm & Hext & Hstorebl & Hdisj & Hstore). *)
+(*   1-3: done. *)
+(*   destruct (deserialize_ML_outcome χ1 ov) as (χ2 & ζimm & lv & Hext2 & Hvs). *)
+(*   1: apply Hext. *)
+(**)
+(*   assert (ζML ρml ∪ ζσ ∪ ζσimm ##ₘ ζimm) as Hdis1. *)
+(*   1: { eapply map_disjoint_dom. eapply disjoint_weaken. 1: eapply Hext2. 2: done. *)
+(*        rewrite dom_union_L. eapply union_subseteq. split. 2: by eapply extended_to_dom_subset. *)
+(*        rewrite dom_union_L. eapply union_subseteq; split. *)
+(*        1: etransitivity; first by eapply elem_of_subseteq. 1: eapply subseteq_dom, Hext. *)
+(*        intros γ Hγ. destruct Hstorebl as [_ HR]. apply HR in Hγ. destruct Hγ as (ℓ & ? & HH & _); by eapply elem_of_dom_2. } *)
+(**)
+(*   pose (ζML ρml ∪ ζσ ∪ (ζσimm ∪ ζimm)) as ζC. *)
+(**)
+(*   destruct (collect_dom_θ_ζ ∅ ζC) as (θdom1 & Hθdom1). *)
+(*   destruct (collect_dom_θ_v θdom1 lv) as (θdom2 & Hθdom2). *)
+(*   destruct (collect_dom_θ_roots θdom2 (rootsML ρml)) as (θdom3 & Hθdom3). *)
+(*   destruct (injectivify_map θdom3) as (θC & Hdom & Hinj). *)
+(*   destruct (find_repr_lval_vv θC lv) as (ws & Hws). *)
+(*   1: intros γ Hγ; subst θdom3; apply Hθdom3; right; apply Hθdom2; left; done. *)
+(*   assert (roots_are_live θC (rootsML ρml)) as Hrootslive. *)
+(*   1: { intros a γ ?. subst θdom3. apply Hθdom3. left. by eexists. } *)
+(*   destruct (find_repr_roots θC (rootsML ρml) (privmemML ρml)) as (mem & Hrepr); [done..|]. *)
+(**)
+(*   pose (match ov with OVal v => OVal ws end) as ow. *)
+(*   eexists ow, (WrapstateC χ2 ζC θC _), mem. *)
+(*   eapply HY. *)
+(*   { exists lv. destruct ov; cbn; split_and; cbn; try done. *)
+(*     eapply is_val_mono; last done; first done. *)
+(*     unfold ζC. rewrite !map_union_assoc. eapply map_union_subseteq_r. done. } *)
+(*   exists ζσ, (ζσimm ∪ ζimm). split_and!; try done; cbn. *)
+(*   { eapply extended_to_trans; done. } *)
+(*   { destruct Hstorebl as [HL HR]; split. *)
+(*     { intros ℓ  Hℓ. destruct (HL ℓ Hℓ) as (γ & Hγ). exists γ. eapply lookup_weaken; first done. apply Hext2. } *)
+(*     { intros γ; destruct (HR γ) as [HRL HRH]; split. *)
+(*        1: intros H; destruct (HRL H) as (ℓ & Vs & H1 & H2); exists ℓ, Vs; split; try done; eapply lookup_weaken; first done; apply Hext2. *)
+(*        intros (ℓ & Vs & H1 & H2). apply HRH. exists ℓ, Vs. split; try done. eapply elem_of_dom_2 in H2. destruct (HL _ H2) as (γ2 & Hγ2). *)
+(*        enough (γ2 = γ) as -> by done. eapply Hext2. 2,3: done. eapply lookup_weaken; first done; eapply Hext2. } } *)
+(*   { intros γ. rewrite dom_union_L. intros [H|H]%elem_of_union; eapply lookup_weaken. *)
+(*     1: by eapply Hext. 2: by eapply Hext2. 2: done. 1: apply Hext2. } *)
+(*   { rewrite map_union_assoc. apply map_disjoint_union_r_2. 1: done. *)
+(*     eapply map_disjoint_dom, disjoint_weaken; first eapply map_disjoint_dom, Hdis1; try done. *)
+(*     erewrite ! dom_union_L; set_solver. } *)
+(*   { intros ℓ vs' γ b H1 H2 H3. unfold ζC in *. rewrite ! map_union_assoc. rewrite ! map_union_assoc in H3. *)
+(*     apply lookup_union_Some_inv_l in H3. *)
+(*     2: apply not_elem_of_dom; intros Hc; apply Hext2 in Hc; congruence. *)
+(*     eapply is_heap_elt_weaken. 1: eapply Hstore; try done. *)
+(*     2: apply Hext2. *)
+(*     + destruct Hstorebl as [HL HR]; destruct (HL ℓ) as [v Hv]; first by eapply elem_of_dom_2. *)
+(*       rewrite <- Hv; f_equal; eapply Hext2; try done; eapply lookup_weaken, Hext2; try done. *)
+(*     + eapply map_union_subseteq_l. } *)
+(*   { split; first done. subst θdom3. intros γ blk γ' _ H2 H3. *)
+(*     apply Hθdom3. right. apply Hθdom2. right. apply Hθdom1. right. left. do 2 eexists; done. } *)
+(* Qed. *)
 
 (* Note: The "freezing step" does properly forbid freezing a
    mutable block that has already been passed to the outside world --- but
@@ -302,24 +316,8 @@ Definition c_to_ml_vals
   (vs : list val) (ρml : wrapstateML) (ζ : lstore)
 : Prop :=
   ∃ lvs,
-    (** Angelically pick a block-level values lvs that corresponds to the
-       C values ws. *)
     Forall2 (repr_lval (θC ρc)) lvs ws ∧
-    (** Angelically pick an ML values vs that correspond to the
-       block-level values lvs. *)
     Forall2 (is_val (χML ρml) ζ) vs lvs.
-
-Definition c_to_ml_val
-  (w : word) (ρc : wrapstateC)
-  (v : val) (ρml : wrapstateML) (ζ : lstore)
-: Prop :=
-  ∃ lv,
-    (** Angelically pick a block-level value lv that corresponds to the
-       C value w. *)
-    repr_lval (θC ρc) lv w ∧
-    (** Angelically pick an ML value v that correspond to the
-       block-level value lv. *)
-    is_val (χML ρml) ζ v lv.
 
 Definition c_to_ml_outcome
   (ow : outcome word) (ρc : wrapstateC)
@@ -538,7 +536,7 @@ Inductive prim_step_mrel (p : prog) : expr * state → (expr * state → Prop) �
   | MakeCallS eml K ρml fn_name vs k σ X :
     is_ML_call eml fn_name vs k →
     p !! fn_name = None →
-    check_ml_state ρml σ →
+    sanity_check ρml σ →
     (∀ ws ρc mem,
        ml_to_c_heap ρml σ ρc mem →
        ml_to_c_vals vs ws ρc →
@@ -547,7 +545,7 @@ Inductive prim_step_mrel (p : prog) : expr * state → (expr * state → Prop) �
   (** Execution finishes with an ML value, translate it into a C value *)
   | OutS eml K ρml σ ov X :
     language.to_outcome eml = Some ov →
-    check_ml_state ρml σ →
+    sanity_check ρml σ →
     (∀ ow ρc mem,
        ml_to_c_heap ρml σ ρc mem →
        ml_to_c_outcome ov ow ρc →
